src/main/scala/qrhl/tactic/IsabelleTac.scala
@@ -8,17 +8,20 @@ import qrhl.logic.Expression
 import qrhl.toplevel.Parser
 
 
-abstract class IsabelleTac[A](operation : Operation[(A, Term, BigInt), Option[List[Term]]], arg : Isabelle.Context => A) extends Tactic {
+abstract class IsabelleTac[A](operation : Operation[(A, Term, BigInt), Option[(List[Term],BigInt)]], arg : Isabelle.Context => A) extends Tactic {
   override def apply(state: State, goal: Subgoal): List[Subgoal] = {
     val ctx = state.isabelle
 //    println("IsabelleTac",Isabelle.pretty(goal.toExpression(ctx).isabelleTerm))
-    val goals = ctx.isabelle.invoke(operation, (arg(ctx), goal.toExpression(ctx).isabelleTerm, ctx.contextId)).getOrElse {
-      throw UserException("tactic failed")
-    }
-//println("IsabelleTac goals",goals.map(Isabelle.pretty))
+    val (goals,thmId) = ctx.isabelle.invoke(operation, (arg(ctx), goal.toExpression(ctx).isabelleTerm, ctx.contextId)).getOrElse {
+      throw UserException("tactic failed") }
+    val thm = if (thmId==0) null else new Isabelle.Thm(ctx.isabelle, thmId)
+
     val newGoals = for (t <- goals) yield Subgoal(ctx, Expression(Isabelle.boolT, t))
-//println("IsabelleTac newGoals",newGoals)
+
     check(state, goal, newGoals)
+
+    if (thm!=null) Subgoal.printOracles(thm)
+
     newGoals
   }
 
