isabelle-thys/Bounded_Operators.thy
@@ -1,5 +1,5 @@
 theory Bounded_Operators
-  imports Complex_L2 "HOL-Library.Adhoc_Overloading"
+  imports Complex_L2 "HOL-Library.Adhoc_Overloading" Extended_Sorry
 begin
 
 
@@ -22,41 +22,38 @@ end
 (* lift_definition timesOp :: "('b,'c) bounded \<Rightarrow> ('a,'b) bounded \<Rightarrow> ('a,'c) bounded" is "(o)"
   unfolding bounded_linear_def unfolding linear_def linear_axioms_def *)
 
-axiomatization
+consts
   adjoint :: "('a,'b) bounded \<Rightarrow> ('b,'a) bounded" ("_*" [99] 100)
-and timesOp :: "('b,'c) bounded \<Rightarrow> ('a,'b) bounded \<Rightarrow> ('a,'c) bounded" 
+ timesOp :: "('b,'c) bounded \<Rightarrow> ('a,'b) bounded \<Rightarrow> ('a,'c) bounded" 
 (* and applyOp :: "('a,'b) bounded \<Rightarrow> 'a vector \<Rightarrow> 'b vector" *)
-and applyOpSpace :: "('a,'b) bounded \<Rightarrow> 'a subspace \<Rightarrow> 'b subspace"
-and timesScalarOp :: "complex \<Rightarrow> ('a,'b) bounded \<Rightarrow> ('a,'b) bounded"
-and timesScalarSpace :: "complex \<Rightarrow> 'a subspace \<Rightarrow> 'a subspace"
-where
- applyOp_0[simp]: "applyOpSpace U 0 = 0"
-and times_applyOp: "applyOp (timesOp A B) \<psi> = applyOp A (applyOp B \<psi>)"
-and timesScalarSpace_0[simp]: "timesScalarSpace 0 S = 0"
-and timesScalarSpace_not0[simp]: "a \<noteq> 0 \<Longrightarrow> timesScalarSpace a S = S"
-and one_times_op[simp]: "timesScalarOp (1::complex) B = B"
+ applyOpSpace :: "('a,'b) bounded \<Rightarrow> 'a subspace \<Rightarrow> 'b subspace"
+ timesScalarOp :: "complex \<Rightarrow> ('a,'b) bounded \<Rightarrow> ('a,'b) bounded"
+ timesScalarSpace :: "complex \<Rightarrow> 'a subspace \<Rightarrow> 'a subspace"
 
-axiomatization where scalar_times_adj[simp]: "(timesScalarOp a A)* = timesScalarOp (cnj a) (A*)" for A::"('a,'b)bounded"
+lemma applyOp_0[simp]: "applyOpSpace U 0 = 0" by (cheat "applyOp_0")
+lemma times_applyOp: "applyOp (timesOp A B) \<psi> = applyOp A (applyOp B \<psi>)" by (cheat times_applyOp)
+lemma timesScalarSpace_0[simp]: "timesScalarSpace 0 S = 0" by (cheat timesScalarSpace_0)
+lemma timesScalarSpace_not0[simp]: "a \<noteq> 0 \<Longrightarrow> timesScalarSpace a S = S" by (cheat timesScalarSpace_not0)
+lemma one_times_op[simp]: "timesScalarOp (1::complex) B = B" by (cheat one_times_op)
+lemma scalar_times_adj[simp]: "(timesScalarOp a A)* = timesScalarOp (cnj a) (A*)" for A::"('a,'b)bounded" by (cheat scalar_times_adj)
 
-axiomatization where
-  timesOp_assoc: "timesOp (timesOp A B) C = timesOp A (timesOp B C)" 
-and times_adjoint[simp]: "adjoint (timesOp A B) = timesOp (adjoint B) (adjoint A)"
-for A :: "('b,'a) bounded" and B :: "('c,'b) bounded" and C :: "('d,'c) bounded"
+lemma timesOp_assoc: "timesOp (timesOp A B) C = timesOp A (timesOp B C)" by (cheat timesOp_assoc)
+lemma times_adjoint[simp]: "adjoint (timesOp A B) = timesOp (adjoint B) (adjoint A)" by (cheat times_adjoint)
+(* for A :: "('b,'a) bounded" and B :: "('c,'b) bounded" and C :: "('d,'c) bounded" *)
 
-axiomatization where
-  timesOp_assoc_subspace: "applyOpSpace (timesOp A B) S = applyOpSpace A (applyOpSpace B S)"
-for S :: "'a subspace" and B :: "('a,'b) bounded" and A :: "('b,'c) bounded"
+lemma timesOp_assoc_subspace: "applyOpSpace (timesOp A B) S = applyOpSpace A (applyOpSpace B S)" by (cheat timesOp_assoc_subspace)
+(* for S :: "'a subspace" and B :: "('a,'b) bounded" and A :: "('b,'c) bounded" *)
 
 
-
-axiomatization plusOp :: "('a,'b) bounded \<Rightarrow> ('a,'b) bounded \<Rightarrow> ('a,'b) bounded" 
+(* TODO: inline into definition of + in instantiation *)
+consts plusOp :: "('a,'b) bounded \<Rightarrow> ('a,'b) bounded \<Rightarrow> ('a,'b) bounded" 
   (* and uminusOp :: "('a,'b) bounded \<Rightarrow> ('a,'b) bounded" *)
-  where
-  plusOp_assoc: "plusOp (plusOp a b) c = plusOp a (plusOp b c)"
-  and plusOp_comm: "plusOp a b = plusOp b a"
-  and plusOp_0: "plusOp 0 a = a"
-  and plusOp_cancel: "plusOp (uminusOp a) a = 0"
-for a b c :: "('a,'b) bounded"
+  
+lemma plusOp_assoc: "plusOp (plusOp a b) c = plusOp a (plusOp b c)" by (cheat plusOp_assoc)
+lemma plusOp_comm: "plusOp a b = plusOp b a" by (cheat plusOp_comm)
+lemma plusOp_0: "plusOp 0 a = a" by (cheat plusOp_0)
+lemma plusOp_cancel: "plusOp (timesScalarOp (-1) a) a = 0" by (cheat plusOp_cancel)
+(* for a b c :: "('a,'b) bounded" *)
 
 lemmas assoc_left = timesOp_assoc[symmetric] timesOp_assoc_subspace[symmetric] plusOp_assoc[symmetric]
 lemmas assoc_right = timesOp_assoc timesOp_assoc_subspace plusOp_assoc
@@ -74,54 +71,62 @@ instance apply intro_classes
   by auto
 end
 
-axiomatization where scalar_times_op_add[simp]: "timesScalarOp a (A+B) = timesScalarOp a A + timesScalarOp a B" for a::complex and A B :: "('a,'b) bounded"
+lemma scalar_times_op_add[simp]: "timesScalarOp a (A+B) = timesScalarOp a A + timesScalarOp a B" for a::complex and A B :: "('a,'b) bounded"
+  by (cheat scalar_times_op_add)
 lemma scalar_times_op_minus[simp]: "timesScalarOp a (A-B) = timesScalarOp a A - timesScalarOp a B" for a::complex and A B :: "('a,'b) bounded"
-  by (metis add_diff_cancel_right' diff_add_cancel scalar_times_op_add)
+  by (cheat TODO1)
 
 lemma applyOp_bot[simp]: "applyOpSpace U bot = bot"
   by (simp add: subspace_zero_bot[symmetric])
 
-axiomatization where equal_basis: "(\<And>x. applyOp A (ket x) = applyOp B (ket x)) \<Longrightarrow> A = B" for A::"('a,'b) bounded"
+lemma equal_basis: "(\<And>x. applyOp A (ket x) = applyOp B (ket x)) \<Longrightarrow> A = B" for A::"('a,'b) bounded"
+  (* apply (tactic  \<open>Extended_Sorry.marked_sorry_tac \<^context> {position= @{here}, comment="xxx"} 1\<close>) *)
+  (* apply (cheat equal_basis) *)
+  sorry
 
-axiomatization where adjoint_twice[simp]: "(U*)* = U" for U :: "('a,'b) bounded"
+lemma adjoint_twice[simp]: "(U*)* = U" for U :: "('a,'b) bounded" by (cheat adjoint_twice)
 
 (* TODO: move specialized syntax into QRHL-specific file *)
 consts cdot :: "'a \<Rightarrow> 'b \<Rightarrow> 'c" (infixl "\<cdot>" 70)
 adhoc_overloading
   cdot timesOp applyOp applyOpSpace timesScalarOp timesScalarSpace timesScalarVec
 
-axiomatization where
-  cdot_plus_distrib[simp]: "U \<cdot> (A + B) = U \<cdot> A + U \<cdot> B"
-for A B :: "'a subspace" and U :: "('a,'b) bounded"
+lemma cdot_plus_distrib[simp]: "U \<cdot> (A + B) = U \<cdot> A + U \<cdot> B"
+  for A B :: "'a subspace" and U :: "('a,'b) bounded"
+  by (cheat cdot_plus_distrib)
 
-axiomatization where scalar_op_subspace_assoc [simp]: 
+lemma scalar_op_subspace_assoc [simp]: 
   "(\<alpha>\<cdot>A)\<cdot>S = \<alpha>\<cdot>(A\<cdot>S)" for \<alpha>::complex and A::"('a,'b)bounded" and S::"'a subspace"
+  by (cheat scalar_op_subspace_assoc)
 
 lemma apply_idOp[simp]: "applyOp idOp \<psi> = \<psi>"
   by (simp add: idOp.rep_eq)
 
-axiomatization where scalar_mult_1_op[simp]: "1 \<cdot> A = A" for A::"('a,'b)bounded"
-axiomatization where scalar_mult_0_op[simp]: "(0::complex) \<cdot> A = 0" for A::"('a,'b)bounded" 
-axiomatization where scalar_op_op[simp]: "(a \<cdot> A) \<cdot> B = a \<cdot> (A \<cdot> B)" 
-  for a :: complex and A :: "('a,'b) bounded" and B :: "('c,'a) bounded"
-axiomatization where op_scalar_op[simp]: "A \<cdot> (a \<cdot> B) = a \<cdot> (A \<cdot> B)" 
-  for a :: complex and A :: "('a,'b) bounded" and B :: "('c,'a) bounded" 
-axiomatization where scalar_scalar_op[simp]: "a \<cdot> (b \<cdot> A) = (a*b) \<cdot> A"
-  for a b :: complex and A  :: "('a,'b) bounded" 
-axiomatization where scalar_op_vec[simp]: "(a \<cdot> A) \<cdot> \<psi> = a \<cdot> (A \<cdot> \<psi>)" 
-  for a :: complex and A :: "('a,'b) bounded" and \<psi> :: "'a vector" 
-axiomatization where add_scalar_mult: "a\<noteq>0 \<Longrightarrow> a \<cdot> A = a \<cdot> B \<Longrightarrow> A=B" for A B :: "('a,'b)bounded" and a::complex 
+lemma scalar_mult_1_op[simp]: "1 \<cdot> A = A" for A::"('a,'b)bounded" by (cheat scalar_mult_1_op)
+lemma scalar_mult_0_op[simp]: "(0::complex) \<cdot> A = 0" for A::"('a,'b)bounded" by (cheat scalar_mult_0_op)
+lemma scalar_op_op[simp]: "(a \<cdot> A) \<cdot> B = a \<cdot> (A \<cdot> B)" 
+  for a :: complex and A :: "('a,'b) bounded" and B :: "('c,'a) bounded" by (cheat scalar_op_op)
+lemma op_scalar_op[simp]: "A \<cdot> (a \<cdot> B) = a \<cdot> (A \<cdot> B)" 
+  for a :: complex and A :: "('a,'b) bounded" and B :: "('c,'a) bounded" by (cheat op_scalar_op)
+lemma scalar_scalar_op[simp]: "a \<cdot> (b \<cdot> A) = (a*b) \<cdot> A"
+  for a b :: complex and A  :: "('a,'b) bounded" by (cheat scalar_scalar_op)
+lemma scalar_op_vec[simp]: "(a \<cdot> A) \<cdot> \<psi> = a \<cdot> (A \<cdot> \<psi>)" 
+  for a :: complex and A :: "('a,'b) bounded" and \<psi> :: "'a vector" by (cheat scalar_op_vec)
+lemma add_scalar_mult: "a\<noteq>0 \<Longrightarrow> a \<cdot> A = a \<cdot> B \<Longrightarrow> A=B" for A B :: "('a,'b)bounded" and a::complex 
+  by (cheat add_scalar_mult)
 
-axiomatization where
+lemma
     apply_idOp_space[simp]: "applyOpSpace idOp S = S"
 and apply_0[simp]: "applyOp U 0 = 0"
 and times_idOp1[simp]: "U \<cdot> idOp = U"
 and times_idOp2[simp]: "idOp \<cdot> V = V"
 and idOp_adjoint[simp]: "idOp* = idOp"
 for \<psi> :: "'a vector" and S :: "'a subspace" and U :: "('a,'b) bounded" and V :: "('b,'a) bounded"
+  sorry
 
-axiomatization where mult_INF[simp]: "U \<cdot> (INF x. V x) = (INF x. U \<cdot> V x)" 
+lemma mult_INF[simp]: "U \<cdot> (INF x. V x) = (INF x. U \<cdot> V x)" 
   for V :: "'a \<Rightarrow> 'b subspace" and U :: "('b,'c) bounded"
+  by (cheat mult_INF)
 
 lemma mult_inf_distrib[simp]: "U \<cdot> (B \<sqinter> C) = (U \<cdot> B) \<sqinter> (U \<cdot> C)" 
   for U :: "('a,'b) bounded" and B C :: "'a subspace"
@@ -167,12 +172,14 @@ proof (unfold inj_option_def, rule allI, rule allI, rule impI, erule conjE)
 qed
 
 
-axiomatization classical_operator :: "('a\<Rightarrow>'b option) \<Rightarrow> ('a,'b) bounded" where
- classical_operator_basis: "inj_option \<pi> \<Longrightarrow>
+consts classical_operator :: "('a\<Rightarrow>'b option) \<Rightarrow> ('a,'b) bounded"
+lemma classical_operator_basis: "inj_option \<pi> \<Longrightarrow>
     applyOp (classical_operator \<pi>) (ket x) = (case \<pi> x of Some y \<Rightarrow> ket y | None \<Rightarrow> 0)"
-axiomatization where classical_operator_adjoint[simp]: 
+  by (cheat TODO5)
+lemma classical_operator_adjoint[simp]: 
   "inj_option \<pi> \<Longrightarrow> adjoint (classical_operator \<pi>) = classical_operator (inv_option \<pi>)"
 for \<pi> :: "'a \<Rightarrow> 'b option"
+  by (cheat TODO1)
 
 
 lemma classical_operator_mult[simp]:
@@ -256,14 +263,16 @@ qed
 
 
 
-axiomatization where unitary_image[simp]: "unitary U \<Longrightarrow> applyOpSpace U top = top"
+lemma unitary_image[simp]: "unitary U \<Longrightarrow> applyOpSpace U top = top"
   for U :: "('a,'a) bounded"
+  by (cheat TODO1)
 
 lemma unitary_id[simp]: "unitary idOp"
   unfolding unitary_def by simp
 
-axiomatization vector_to_bounded :: "'a vector \<Rightarrow> (unit,'a) bounded"
-  where vector_to_bounded_applyOp: "vector_to_bounded (A\<cdot>\<psi>) = A \<cdot> vector_to_bounded \<psi>" for A :: "(_,_)bounded"
+consts vector_to_bounded :: "'a vector \<Rightarrow> (unit,'a) bounded"
+lemma vector_to_bounded_applyOp: "vector_to_bounded (A\<cdot>\<psi>) = A \<cdot> vector_to_bounded \<psi>" for A :: "(_,_)bounded"
+  by (cheat TODO5)
 
 lemma vector_to_bounded_scalar_times: "vector_to_bounded (a\<cdot>\<psi>) = a \<cdot> vector_to_bounded \<psi>" for a::complex
   apply (rewrite at "a\<cdot>\<psi>" DEADID.rel_mono_strong[of _ "(a\<cdot>idOp)\<cdot>\<psi>"])
@@ -272,15 +281,18 @@ lemma vector_to_bounded_scalar_times: "vector_to_bounded (a\<cdot>\<psi>) = a \<
   by simp
 
 
-axiomatization kernel :: "('a,'b) bounded \<Rightarrow> 'a subspace"
+consts kernel :: "('a,'b) bounded \<Rightarrow> 'a subspace"
 definition eigenspace :: "complex \<Rightarrow> ('a,'a) bounded \<Rightarrow> 'a subspace" where
   "eigenspace a A = kernel (A-a\<cdot>idOp)" 
 
-axiomatization where kernel_scalar_times[simp]: "a\<noteq>0 \<Longrightarrow> kernel (a\<cdot>A) = kernel A" 
+lemma kernel_scalar_times[simp]: "a\<noteq>0 \<Longrightarrow> kernel (a\<cdot>A) = kernel A" 
   for a :: complex and A :: "('a,'b) bounded"
+  by (cheat TODO1)
 
-axiomatization where kernel_0[simp]: "kernel 0 = top"
-axiomatization where kernel_id[simp]: "kernel idOp = 0"
+lemma kernel_0[simp]: "kernel 0 = top"
+  by (cheat TODO1)
+lemma kernel_id[simp]: "kernel idOp = 0"
+  by (cheat TODO1)
 
 lemma [simp]: "a\<noteq>0 \<Longrightarrow> eigenspace b (a\<cdot>A) = eigenspace (b/a) A"
   unfolding eigenspace_def
@@ -294,44 +306,53 @@ section \<open>Projectors\<close>
 
 definition "isProjector P = (P=P* \<and> P=P\<cdot>P)"
 
-axiomatization Proj :: "'a subspace \<Rightarrow> ('a,'a) bounded" where
-  isProjector_Proj[simp]: "isProjector (Proj S)"
-and imageOp_Proj[simp]: "applyOpSpace (Proj S) top = S"
+consts Proj :: "'a subspace \<Rightarrow> ('a,'a) bounded"
+lemma isProjector_Proj[simp]: "isProjector (Proj S)"
+  by (cheat TODO5)
+
+lemma imageOp_Proj[simp]: "applyOpSpace (Proj S) top = S"
+  by (cheat TODO5)
 
 lemma Proj_leq: "Proj S \<cdot> A \<le> S"
   by (metis imageOp_Proj inf.orderE inf.orderI mult_inf_distrib top_greatest)
 
 
-axiomatization where Proj_times: "A \<cdot> Proj S \<cdot> A* = Proj (A\<cdot>S)" for A::"('a,'b)bounded"
+lemma Proj_times: "A \<cdot> Proj S \<cdot> A* = Proj (A\<cdot>S)" for A::"('a,'b)bounded"
+  by (cheat TODO2)
 
 abbreviation proj :: "'a vector \<Rightarrow> ('a,'a) bounded" where "proj \<psi> \<equiv> Proj (span {\<psi>})"
 
-axiomatization where proj_scalar_mult[simp]: 
+lemma proj_scalar_mult[simp]: 
   "a \<noteq> 0 \<Longrightarrow> proj (a \<cdot> \<psi>) = proj \<psi>" for a::complex and \<psi>::"'a vector"
+  by (cheat TODO2)
 
 
-axiomatization where move_plus:
+lemma move_plus:
   "Proj (ortho C) \<cdot> A \<le> B \<Longrightarrow> A \<le> B + C"
 for A B C::"'a subspace"
+  by (cheat TODO2)
 
 
 section \<open>Tensor products\<close>
 
-axiomatization "tensorOp" :: "('a,'b) bounded \<Rightarrow> ('c,'d) bounded \<Rightarrow> ('a*'c,'b*'d) bounded"
-axiomatization "tensorSpace" :: "'a subspace \<Rightarrow> 'c subspace \<Rightarrow> ('a*'c) subspace"
-axiomatization "tensorVec" :: "'a vector \<Rightarrow> 'c vector \<Rightarrow> ('a*'c) vector"
+consts "tensorOp" :: "('a,'b) bounded \<Rightarrow> ('c,'d) bounded \<Rightarrow> ('a*'c,'b*'d) bounded"
+consts "tensorSpace" :: "'a subspace \<Rightarrow> 'c subspace \<Rightarrow> ('a*'c) subspace"
+consts "tensorVec" :: "'a vector \<Rightarrow> 'c vector \<Rightarrow> ('a*'c) vector"
 consts tensor :: "'a \<Rightarrow> 'b \<Rightarrow> 'c" (infix "\<otimes>" 71)
 adhoc_overloading tensor tensorOp tensorSpace tensorVec
 
-axiomatization where idOp_tensor_idOp[simp]: "idOp\<otimes>idOp = idOp"
+lemma idOp_tensor_idOp[simp]: "idOp\<otimes>idOp = idOp"
+  by (cheat TODO2)
 
-axiomatization "comm_op" :: "('a*'b, 'b*'a) bounded"
+consts "comm_op" :: "('a*'b, 'b*'a) bounded"
 
-axiomatization where adj_comm_op[simp]: "adjoint comm_op = comm_op"
+lemma adj_comm_op[simp]: "adjoint comm_op = comm_op"
+  by (cheat TODO2)
 
-axiomatization where
+lemma
   comm_op_swap[simp]: "comm_op \<cdot> (A\<otimes>B) \<cdot> comm_op = B\<otimes>A"
   for A::"('a,'b) bounded" and B::"('c,'d) bounded"
+  by (cheat TODO3)
 
 lemma comm_op_times_comm_op[simp]: "comm_op \<cdot> comm_op = idOp"
 proof -
@@ -343,17 +364,21 @@ qed
 lemma unitary_comm_op[simp]: "unitary comm_op"
   unfolding unitary_def by simp
 
-axiomatization "assoc_op" :: "('a*'b*'c, ('a*'b)*'c) bounded"
-  where unitary_assoc_op[simp]: "unitary assoc_op"
+consts "assoc_op" :: "('a*'b*'c, ('a*'b)*'c) bounded"
+lemma unitary_assoc_op[simp]: "unitary assoc_op"
+  by (cheat TODO5)
 
-axiomatization where tensor_scalar_mult1[simp]: "(a \<cdot> A) \<otimes> B = a \<cdot> (A \<otimes> B)" for a::complex and A::"('a,'b)bounded" and B::"('c,'d)bounded"
-axiomatization where tensor_scalar_mult2[simp]: "A \<otimes> (a \<cdot> B) = a \<cdot> (A \<otimes> B)" for a::complex and A::"('a,'b)bounded" and B::"('c,'d)bounded"
+lemma tensor_scalar_mult1[simp]: "(a \<cdot> A) \<otimes> B = a \<cdot> (A \<otimes> B)" for a::complex and A::"('a,'b)bounded" and B::"('c,'d)bounded"
+  by (cheat TODO3)
+lemma tensor_scalar_mult2[simp]: "A \<otimes> (a \<cdot> B) = a \<cdot> (A \<otimes> B)" for a::complex and A::"('a,'b)bounded" and B::"('c,'d)bounded"
+  by (cheat TODO3)
 
-axiomatization where tensor_times[simp]: "(U1 \<otimes> U2) \<cdot> (V1 \<otimes> V2) = (U1 \<cdot> V1) \<otimes> (U2 \<cdot> V2)"
+lemma tensor_times[simp]: "(U1 \<otimes> U2) \<cdot> (V1 \<otimes> V2) = (U1 \<cdot> V1) \<otimes> (U2 \<cdot> V2)"
   for V1 :: "('a1,'b1) bounded" and U1 :: "('b1,'c1) bounded"
    and V2 :: "('a2,'b2) bounded" and U2 :: "('b2,'c2) bounded"
+  by (cheat TODO3)
 
-axiomatization remove_qvar_unit_op :: "('a*unit,'a) bounded"
+consts remove_qvar_unit_op :: "('a*unit,'a) bounded"
 
 
 definition addState :: "'a vector \<Rightarrow> ('b,'b*'a) bounded" where
@@ -362,8 +387,9 @@ definition addState :: "'a vector \<Rightarrow> ('b,'b*'a) bounded" where
 lemma addState_times_scalar[simp]: "addState (a \<cdot> \<psi>) = a \<cdot> addState \<psi>" for a::complex and psi::"'a vector"
   unfolding addState_def by (simp add: vector_to_bounded_scalar_times)
 
-axiomatization where tensor_adjoint[simp]: "adjoint (U\<otimes>V) = (adjoint U) \<otimes> (adjoint V)"
+lemma tensor_adjoint[simp]: "adjoint (U\<otimes>V) = (adjoint U) \<otimes> (adjoint V)"
   for U :: "('a,'b) bounded" and V :: "('c,'d) bounded"
+  by (cheat TODO3)
 
 
 lemma tensor_unitary[simp]: 
